pi homomorphisme

ocaml/quicksort2.ml
@@ -1,0 +1,53 @@
+
+(** val app : 'a1 list -> 'a1 list -> 'a1 list **)
+
+let rec app l m =
+  match l with
+  | [] -> m
+  | a :: l1 -> a :: (app l1 m)
+
+(** val leb : int -> int -> bool **)
+
+let rec leb n m =
+  (fun fO fS n -> if n=0 then fO () else fS (n-1))
+    (fun _ -> true)
+    (fun n' ->
+    (fun fO fS n -> if n=0 then fO () else fS (n-1))
+      (fun _ -> false)
+      (fun m' -> leb n' m')
+      m)
+    n
+
+(** val ltb : int -> int -> bool **)
+
+let ltb n m =
+  leb (Pervasives.succ n) m
+
+(** val filter : ('a1 -> bool) -> 'a1 list -> 'a1 list **)
+
+let rec filter f = function
+| [] -> []
+| x :: l0 -> if f x then x :: (filter f l0) else filter f l0
+
+(** val flip_ltb : int -> int -> bool **)
+
+let flip_ltb x y =
+  ltb y x
+
+(** val flip_geb : int -> int -> bool **)
+
+let flip_geb =
+  leb
+
+(** val quickSort' : int list -> int list **)
+
+let rec quickSort' = function
+| [] -> []
+| x :: xs ->
+  app (quickSort' (filter (flip_ltb x) xs))
+    (x :: (quickSort' (filter (flip_geb x) xs)))
+
+(** val quickSort : int list -> int list **)
+
+let quickSort =
+  quickSort'
