quicksort.ml
@@ -1,0 +1,49 @@
+
+(** val negb : bool -> bool **)
+
+let negb = function
+| true -> false
+| false -> true
+
+(** val app :
+    'a1 list -> 'a1 list -> 'a1 list **)
+
+let rec app l m =
+  match l with
+  | [] -> m
+  | a :: l1 -> a :: (app l1 m)
+
+module Nat =
+ struct
+ end
+
+(** val filter :
+    ('a1 -> bool) -> 'a1 list -> 'a1 list **)
+
+let rec filter f = function
+| [] -> []
+| x :: l0 ->
+  if f x
+  then x :: (filter f l0)
+  else filter f l0
+
+(** val filter_lte :
+    int -> int list -> int list **)
+
+let filter_lte a list0 =
+  filter (fun n -> (<=) n a) list0
+
+(** val filter_gt :
+    int -> int list -> int list **)
+
+let filter_gt a list0 =
+  filter (fun n -> negb ((<=) n a)) list0
+
+(** val quicksort : int list -> int list **)
+
+let rec quicksort = function
+| [] -> []
+| h :: t ->
+  let sorted_t = quicksort t in
+  app (filter_lte h sorted_t)
+    (h :: (filter_gt h sorted_t))
