quicksort.mli
@@ -1,0 +1,17 @@
+
+val negb : bool -> bool
+
+val app : 'a1 list -> 'a1 list -> 'a1 list
+
+module Nat :
+ sig
+ end
+
+val filter :
+  ('a1 -> bool) -> 'a1 list -> 'a1 list
+
+val filter_lte : int -> int list -> int list
+
+val filter_gt : int -> int list -> int list
+
+val quicksort : int list -> int list
