ret_num.ml
@@ -1,0 +1,5 @@
+
+(** val ret_num : int -> int **)
+
+let ret_num n =
+  n
