ret_num.mli
@@ -1,0 +1,2 @@
+
+val ret_num : int -> int
