ocaml/quicksort.v
@@ -1,0 +1,118 @@
+Require Import List.
+Require Import Bool.
+Require Import Arith.
+
+Require Extraction.
+Require Import ExtrOcamlNatInt.
+
+Definition filter_lte (a: nat) list := filter (fun n=> n <=? a) list.
+Definition filter_gt (a: nat) list := filter (fun n=> negb(n <=? a)) list.
+
+Fixpoint quicksort (l: list nat) :=
+    match l with
+      nil => nil
+    | h :: t => let sorted_t := quicksort t in
+                    filter_lte h sorted_t
+                    ++ h :: filter_gt h sorted_t
+    end.
+
+Compute quicksort (nil).
+Compute quicksort (1::2::3::6::1::2::1::0::nil).
+
+Fixpoint length (l: list nat) : nat :=
+    match l with
+      nil => 0
+    | a :: tl => 1 + (length (tl))
+    end.
+
+Theorem lengthIsCommutative: forall l m : list nat, length(l ++ m) = length(m ++ l).
+Proof.
+    induction l.
+    intros.
+    simpl.
+    rewrite app_nil_r.
+    reflexivity.
+    intros.
+    simpl.
+    rewrite IHl.
+    induction m.
+    simpl.
+    reflexivity.
+    simpl.
+    rewrite IHm.
+    reflexivity.
+Qed.
+
+Theorem lengthIsDistributive: forall l j:(list nat), length (l ++ j) = length l + length j.
+Proof.
+    induction j.
+    simpl.
+    rewrite app_nil_r.
+    firstorder.
+    rewrite lengthIsCommutative.
+    simpl.
+    rewrite Nat.add_succ_r with (n:=length l) (m:=length j).
+    rewrite lengthIsCommutative.
+    rewrite IHj.
+    firstorder.
+Qed.
+
+Theorem twoFilterLengthEq: forall n l, length(filter_lte n l) + length(filter_gt n l) = length(l).
+Proof.
+    intros.
+    induction l.
+    simpl.
+    reflexivity.
+    unfold filter_lte.
+    assert ((fun n0 : nat => n0 <=? n) a = true \/ (fun n0 : nat => negb(n0 <=? n)) a = true).
+    case (a <=? n).
+    left; reflexivity.
+    right; simpl; reflexivity.
+    destruct H.
+    simpl.
+    rewrite H.
+    simpl.
+    assert (filter_lte n l = filter (fun n0 : nat => n0 <=? n) l).
+    unfold filter_lte.
+    firstorder.
+    rewrite <- H0.
+    rewrite IHl.
+    firstorder.
+    assert (filter_lte n (a::l) = filter (fun n0 : nat => n0 <=? n) (a::l)).
+    unfold filter_lte.
+    firstorder.
+    rewrite <- H0.
+    simpl.
+    rewrite H.
+    assert((a <=? n) = false).
+    rewrite <- negb_involutive with (b:=(a <=? n)).
+    rewrite H.
+    firstorder.
+    rewrite H1.
+    simpl.
+    rewrite Nat.add_succ_r with (n:=length(filter_lte n l)) (m:=(length (filter_gt n l))).
+    rewrite IHl.
+    firstorder.
+Qed.
+
+Theorem sortLengthUnchanged :
+    forall l:(list nat),
+    length l = length (quicksort l).
+Proof.
+    induction l.
+    simpl.
+    reflexivity.
+    simpl.
+    rewrite IHl.
+    rewrite lengthIsDistributive.
+    simpl.
+    rewrite Nat.add_succ_r with
+        (n:=length(filter_lte a (quicksort l)))
+        (m:=(length (filter_gt a (quicksort l)))).
+    rewrite twoFilterLengthEq.
+    reflexivity.
+Qed.
+
+(* https://gist.github.com/adampalay/44b9ac3515469d92cb2f295e6179b8b9 *)
+
+Extraction "quicksort.ml" quicksort.
