ocaml/quicksort2.v
@@ -1,0 +1,317 @@
+(* Largely inspired by https://github.com/coq/coq/wiki/QuickSort *)
+Require Import Arith.Wf_nat Bool List Nat Lia.
+Require Import Sorting.Permutation Sorting.Sorted.
+
+Definition flip_ltb (x : nat) : nat -> bool :=
+  fun (y : nat) => y <? x.
+
+Definition flip_geb (x : nat) : nat -> bool :=
+  fun (y : nat) => x <=? y.
+
+Inductive QSAcc : list nat -> Prop :=
+| QSAccNil  : QSAcc nil
+| QSAccCons : forall x xs,
+              QSAcc (filter (flip_ltb x) xs) ->
+              QSAcc (filter (flip_geb x) xs) ->
+              QSAcc (x :: xs).
+
+Lemma QSAcc_inv_1 :
+  forall {x xs l},
+  QSAcc l -> l = (x :: xs) ->
+  QSAcc (filter (flip_ltb x) xs).
+Proof. intros. subst. inversion H. auto. Defined.
+
+Lemma QSAcc_inv_2 :
+  forall {x xs l},
+  QSAcc l -> l = (x :: xs) ->
+  QSAcc (filter (flip_geb x) xs).
+Proof. intros. subst. inversion H. auto. Defined.
+
+Fixpoint quickSort' (l : list nat) (acc : QSAcc l) {struct acc} : list nat :=
+  match l as l0 return (l = l0 -> list nat) with
+  | nil =>
+      fun (_ : l = nil) => nil
+  | x :: xs =>
+      fun (H : l = (x :: xs)) =>
+      quickSort' (filter (flip_ltb x) xs) (QSAcc_inv_1 acc H) ++
+      x :: quickSort' (filter (flip_geb x) xs) (QSAcc_inv_2 acc H)
+  end (eq_refl l).
+
+Lemma induction_ltof1_Prop
+     : forall (A : Set) (f : A -> nat) (P : A -> Prop),
+       (forall x : A, (forall y : A, ltof A f y x -> P y) -> P x) ->
+       forall a : A, P a.
+Proof.
+  intros A f P F.
+  assert (H : forall (n : nat) (a : A), f a < n -> P a).
+  { induction n; intros.
+    - omega.
+    - apply F. unfold ltof. intros. apply IHn.
+      apply Nat.lt_le_trans with (m := f a); omega. }
+  intros. apply H with (n := S (f a)). omega.
+Defined.
+
+Lemma filter_length :
+  forall {a} (f : a -> bool) (l : list a),
+  length (filter f l) <= length l.
+Proof.
+  induction l; simpl; auto.
+  destruct (f a0); simpl; auto. omega.
+Defined.
+
+Theorem qsAcc : forall l, QSAcc l.
+Proof.
+  intros. apply (induction_ltof1_Prop _ (@length nat)).
+  intros. destruct x as [|x xs]; constructor; apply H; unfold ltof; simpl.
+  - pose proof (filter_length (flip_ltb x) xs). omega.
+  - pose proof (filter_length (flip_geb x) xs). omega.
+Defined.
+Scheme QSAcc_ind_dep := Induction for QSAcc Sort Prop.
+
+Definition quickSort (l : list nat) : list nat :=
+  quickSort' l (qsAcc l).
+
+Lemma unit_test : quickSort (2 :: 3 :: 1 :: nil) = 1 :: 2 :: 3 :: nil.
+Proof. auto. Qed.
+
+Lemma quickSort'_PI' :
+  forall {l1} (acc1 : QSAcc l1) {l2} (acc2 : QSAcc l2),
+  l1 = l2 ->
+  quickSort' l1 acc1 = quickSort' l2 acc2.
+Proof.
+  apply (QSAcc_ind_dep
+          (fun (l' : list nat) (acc' : QSAcc l') =>
+           forall (l2 : list nat) (acc2 : QSAcc l2),
+           l' = l2 -> quickSort' l' acc' = quickSort' l2 acc2)).
+  - apply (QSAcc_ind_dep
+            (fun (l' : list nat) (acc' : QSAcc l') =>
+             nil = l' ->
+             quickSort' nil QSAccNil = quickSort' l' acc')); try discriminate. auto.
+  - intros until 2.
+    apply (QSAcc_ind_dep
+            (fun (l' : list nat) (acc' : QSAcc l') =>
+             x :: xs = l' ->
+             quickSort' (x :: xs) (QSAccCons x xs q q0) = quickSort' l' acc')); try discriminate.
+    intros. injection H3 as H4 H5. subst. simpl.
+    pose proof (H  (filter (flip_ltb x0) xs0) (QSAcc_inv_1 (QSAccCons x0 xs0 q q0) eq_refl) eq_refl).
+    pose proof (H0 (filter (flip_geb x0) xs0) (QSAcc_inv_2 (QSAccCons x0 xs0 q q0) eq_refl) eq_refl).
+    rewrite <- H3. rewrite <- H4.
+    pose proof (H  (filter (flip_ltb x0) xs0) (QSAcc_inv_1 (QSAccCons x0 xs0 q1 q2) eq_refl) eq_refl).
+    pose proof (H0 (filter (flip_geb x0) xs0) (QSAcc_inv_2 (QSAccCons x0 xs0 q1 q2) eq_refl) eq_refl).
+    rewrite <- H5. rewrite <- H6. auto.
+Qed.
+
+Lemma quickSort'_PI :
+  forall {l} (acc1 acc2 : QSAcc l),
+  quickSort' l acc1 = quickSort' l acc2.
+Proof. intros. rewrite (quickSort'_PI' acc1 acc2); auto. Qed.
+
+Theorem quickSort'_nil :
+  forall (acc : QSAcc nil),
+  quickSort' nil acc = nil.
+Proof. intros. rewrite (quickSort'_PI acc QSAccNil). auto. Qed.
+
+Theorem quickSort_nil :
+  quickSort nil = nil.
+Proof. auto. Qed.
+
+Theorem quickSort'_cons :
+  forall {x xs} (acc   : QSAcc (x :: xs))
+                (accLT : QSAcc (filter (flip_ltb x) xs))
+                (accGE : QSAcc (filter (flip_geb x) xs)),
+  quickSort' (x :: xs) acc =
+    quickSort' (filter (flip_ltb x) xs) accLT ++
+    x :: quickSort' (filter (flip_geb x) xs) accGE.
+Proof. intros. rewrite (quickSort'_PI acc (QSAccCons x xs accLT accGE)). auto. Qed.
+
+Theorem quickSort'_cons_exists :
+  forall {x xs} (acc : QSAcc (x :: xs)),
+  exists (accLT : QSAcc (filter (flip_ltb x) xs))
+         (accGE : QSAcc (filter (flip_geb x) xs)),
+  quickSort' (x :: xs) acc =
+    quickSort' (filter (flip_ltb x) xs) accLT ++
+    x :: quickSort' (filter (flip_geb x) xs) accGE.
+Proof.
+  intros.
+  pose proof (qsAcc (filter (flip_ltb x) xs)) as accLT.
+  pose proof (qsAcc (filter (flip_geb x) xs)) as accGE.
+  exists accLT. exists accGE.
+  rewrite (quickSort'_PI acc (QSAccCons x xs accLT accGE)). auto.
+Qed.
+
+Theorem quickSort_cons_QSAccCons :
+  forall {x xs} (accLT : QSAcc (filter (flip_ltb x) xs))
+                (accGE : QSAcc (filter (flip_geb x) xs)),
+  quickSort' (x :: xs) (QSAccCons x xs accLT accGE) =
+    quickSort' (filter (flip_ltb x) xs) accLT ++
+    x :: quickSort' (filter (flip_geb x) xs) accGE.
+Proof. intros. rewrite (quickSort'_cons _ accLT accGE). auto. Qed.
+
+Theorem quickSort_cons :
+  forall {x xs},
+  quickSort (x :: xs) =
+    quickSort (filter (flip_ltb x) xs) ++
+    x :: quickSort (filter (flip_geb x) xs).
+Proof. intros. unfold quickSort. apply quickSort'_cons. Qed.
+
+Hint Resolve Nat.ltb_spec0 Nat.leb_spec0 Nat.eqb_spec : bdestruct.
+
+Ltac bdestruct X :=
+  let H := fresh in let e := fresh "e" in
+   evar (e: Prop);
+   assert (H: reflect e X); subst e;
+    [eauto with bdestruct
+    | destruct H as [H|H];
+       [ | try first [apply not_lt in H | apply not_le in H]]].
+
+Lemma HdRel_app :
+  forall (a : nat) (c : nat) (bs : list nat) (ds : list nat),
+  a <= c -> HdRel le a bs ->
+  HdRel le a (bs ++ c :: ds).
+Proof.
+  induction bs; simpl; intros.
+  - constructor. auto.
+  - inversion H0. constructor. auto.
+Qed.
+
+Lemma HdRel_extend :
+  forall (a b : nat) (l : list nat),
+  a <= b -> HdRel le b l ->
+  HdRel le a l.
+Proof.
+  intros. destruct l.
+  - auto.
+  - constructor. inversion H0. subst. omega.
+Qed.
+
+Lemma HdRel_filter :
+  forall (a : nat) (f : nat -> bool) (l : list nat),
+  Sorted le l -> HdRel le a l ->
+  HdRel le a (filter f l).
+Proof.
+  intros. induction H; simpl.
+  - auto.
+  - inversion H0. subst. destruct (f a0).
+    + constructor. auto.
+    + apply IHSorted. apply HdRel_extend with (b := a0); auto.
+Qed.
+
+Lemma Sorted_partition :
+  forall (x : nat) (l1 l2 : list nat),
+  Sorted le l1 -> Sorted le l2 ->
+  (forall y, In y l1 -> y <  x) ->
+  (forall y, In y l2 -> x <= y) ->
+  Sorted le (l1 ++ x :: l2).
+Proof.
+  intros until 1. revert l2. induction H; simpl.
+  - intros. constructor; auto. destruct l2.
+    + auto.
+    + constructor. inversion H. subst. apply H1. left. auto.
+  - intros. constructor; auto.
+    assert (AX : a < x). { apply H2. left. auto. }
+    apply HdRel_app.
+    + omega.
+    + auto.
+Qed.
+
+Lemma Sorted_filter :
+  forall (f : nat -> bool) (l : list nat),
+  Sorted le l -> Sorted le (filter f l).
+Proof.
+  intros. induction H; simpl.
+  - auto.
+  - destruct (f a); auto. constructor; auto. apply HdRel_filter; auto.
+Qed.
+
+Lemma In_filter_ltb :
+  forall (x y : nat) (l : list nat),
+  In y (filter (flip_ltb x) l) ->
+  y < x.
+Proof.
+  intros. induction l.
+  - contradiction.
+  - simpl in H. unfold flip_ltb in H. bdestruct (a <? x); auto.
+    simpl in H. destruct H; auto. subst. auto.
+Qed.
+
+Lemma In_filter_geb :
+  forall (x y : nat) (l : list nat),
+  In y (filter (flip_geb x) l) ->
+  x <= y.
+Proof.
+  intros. induction l.
+  - contradiction.
+  - simpl in H. unfold flip_geb in H. bdestruct (x <=? a); auto.
+    simpl in H. destruct H; auto. subst. auto.
+Qed.
+
+Lemma In_quickSort' :
+  forall x l acc,
+  In x (quickSort' l acc) -> In x l.
+Proof.
+  intro x.
+  apply (QSAcc_ind_dep
+          (fun (l' : list nat) (acc' : QSAcc l') =>
+           In x (quickSort' l' acc') -> In x l')).
+  - auto.
+  - intros. rewrite (quickSort_cons_QSAccCons q q0) in H1.
+    simpl. apply in_app_or in H1. destruct H1.
+    + specialize (H H1).
+      pose proof (filter_In (flip_ltb x0) x xs).
+      destruct H2. specialize (H2 H). destruct H2. right. auto.
+    + destruct H1.
+      * left. auto.
+      * specialize (H0 H1).
+        pose proof (filter_In (flip_geb x0) x xs).
+        destruct H2. specialize (H2 H0). destruct H2. right. auto.
+Qed.
+
+Lemma Permutation_filter_ltb_geb :
+  forall (x : nat) (l : list nat),
+  Permutation l (filter (flip_ltb x) l ++ filter (flip_geb x) l).
+Proof.
+  induction l; simpl.
+  - constructor.
+  - unfold flip_ltb, flip_geb.
+    bdestruct (a <? x); bdestruct (x <=? a); try omega.
+    + constructor; auto.
+    + apply Permutation_cons_app. auto.
+Qed.
+
+Theorem quickSort'_Sorted :
+  forall l (acc : QSAcc l),
+  Sorted le (quickSort' l acc).
+Proof.
+  apply (QSAcc_ind_dep
+          (fun (l' : list nat) (acc' : QSAcc l') =>
+           Sorted le (quickSort' l' acc'))).
+  - constructor.
+  - intros. rewrite (quickSort_cons_QSAccCons q q0).
+    apply Sorted_partition; auto; intros.
+    + apply In_quickSort' in H1. apply In_filter_ltb in H1. auto.
+    + apply In_quickSort' in H1. apply In_filter_geb in H1. auto.
+Qed.
+
+Theorem quickSort'_Permutation' :
+  forall l (acc : QSAcc l),
+  Permutation l (quickSort' l acc).
+Proof.
+  apply (QSAcc_ind_dep
+          (fun (l' : list nat) (acc' : QSAcc l') =>
+           Permutation l' (quickSort' l' acc'))).
+  - constructor.
+  - intros. rewrite (quickSort_cons_QSAccCons q q0).
+    apply Permutation_cons_app.
+    apply Permutation_trans with
+      (l' := filter (flip_ltb x) xs ++ filter (flip_geb x) xs).
+    + apply Permutation_filter_ltb_geb.
+    + apply Permutation_app; auto.
+Qed.
+
+Theorem quickSort_correct :
+  forall l,
+  Sorted le (quickSort l) /\ Permutation l (quickSort l).
+Proof. unfold quickSort; split.
+- apply quickSort'_Sorted.
+- apply quickSort'_Permutation'.
+Qed.
