ocaml/ret_num.v
@@ -1,0 +1,5 @@
+Require Extraction.
+Require Import ExtrOcamlNatInt.
+Definition ret_num (n:nat) := n.
+
+Extraction "ret_num.ml" ret_num.
